.

projects/FirstOrderModalLogic.v
@@ -7,63 +7,9 @@ Module FirstOrderModalLogic.
 
   Import ListNotations MyUtilities MyEnsemble.
 
-  Record language_arity_env : Set :=
-    MkArityEnv
-    { func_arity : forall fsym_id : nat, nat
-    ; pred_arity : forall psym_id : nat, nat
-    }
-  .
-
   Definition ivar : Set :=
     nat
   .
-
-  Variant symbol : Set :=
-  | CONTRADICTION : symbol
-  | NEGATION : symbol
-  | CONJUNCTION : symbol
-  | DISJUNCTION : symbol
-  | IMPLICATION : symbol
-  | BICONDITIONAL : symbol 
-  | FORALL : symbol
-  | EXISTS : symbol
-  | EQUAL : symbol
-  | BOX : symbol
-  | DIA : symbol
-  | FuncSym (fsym_id : nat) : symbol
-  | PredSym (psym_id : nat) : symbol
-  .
-
-  Inductive tm : Set :=
-  | VAR (x : ivar) : tm
-  | CON (c : symbol) : tm
-  | APP (t1 : tm) (t2 : tm) : tm
-  | LAM (y : ivar) (t1 : tm) : tm
-  .
-
-  Inductive ty : Set :=
-  | TyI : ty
-  | TyO : ty
-  | ARR (arg_ty : ty) (ret_ty : ty) : ty
-  .
-
-  Global Declare Custom Entry object_level_ty.
-
-  Global Notation " 'i' " := (TyI) (in custom object_level_ty at level 0, no associativity).
-
-  Global Notation " 'o' " := (TyO) (in custom object_level_ty at level 0, no associativity).
-
-  Global Notation " ty1 '->' ty2 " := (ARR ty1 ty2) (in custom object_level_ty at level 1, right associativity).
-
-  Global Notation " ty1 " := (ty1) (in custom object_level_ty, ty1 ident).
-
-  Global Notation " '(' ty1 ')' " := (ty1) (in custom object_level_ty at level 0, no associativity).
-
-  Global Declare Scope object_level_ty_scope.
-
-  Global Notation " '\ty(' ty_expr ')' " := (ty_expr) (ty_expr custom object_level_ty at level 1, at level 0, no associativity) : object_level_ty_scope.
-
-  Local Open Scope object_level_ty_scope.
 
   Definition ivar_eq_dec :
     forall x : ivar,
@@ -72,6 +18,34 @@ Module FirstOrderModalLogic.
   Proof.
     exact (fun x y => Nat.eq_dec x y).
   Defined.
+
+  Variant logical_symbol : Set :=
+  | CONTRADICTION : logical_symbol
+  | NEGATION : logical_symbol
+  | CONJUNCTION : logical_symbol
+  | DISJUNCTION : logical_symbol
+  | IMPLICATION : logical_symbol
+  | BICONDITIONAL : logical_symbol 
+  | FORALL : logical_symbol
+  | EXISTS : logical_symbol
+  | EQUAL : logical_symbol
+  | BOX : logical_symbol
+  | DIA : logical_symbol
+  .
+
+  Definition logical_symbol_eq_dec :
+    forall s1 : logical_symbol,
+    forall s2 : logical_symbol,
+    {s1 = s2} + {s1 <> s2}.
+  Proof.
+    induction s1; destruct s2; ((left; congruence) || (right; congruence)).
+  Defined.
+
+  Inductive ty : Set :=
+  | TyI : ty
+  | TyO : ty
+  | ARR (arg_ty : ty) (ret_ty : ty) : ty
+  .
 
   Definition ty_eq_dec :
     forall ty1 : ty,
@@ -94,10 +68,26 @@ Module FirstOrderModalLogic.
       + right; congruence.
   Defined.
 
-  Section EVALUATION.
+  Global Declare Custom Entry object_level_ty.
 
-  Definition get_ty_of_symbol (arity_env : language_arity_env) (c : symbol) : ty :=
-    match c with
+  Global Notation " 'i' " := (TyI) (in custom object_level_ty at level 0, no associativity).
+
+  Global Notation " 'o' " := (TyO) (in custom object_level_ty at level 0, no associativity).
+
+  Global Notation " ty1 '->' ty2 " := (ARR ty1 ty2) (in custom object_level_ty at level 1, right associativity).
+
+  Global Notation " ty1 " := (ty1) (in custom object_level_ty, ty1 ident).
+
+  Global Notation " '(' ty1 ')' " := (ty1) (in custom object_level_ty at level 0, no associativity).
+
+  Global Declare Scope object_level_ty_scope.
+
+  Global Notation " '\ty(' ty_expr ')' " := (ty_expr) (ty_expr custom object_level_ty at level 1, at level 0, no associativity) : object_level_ty_scope.
+
+  Local Open Scope object_level_ty_scope.
+
+  Definition get_ty_of_logical_symbol (s : logical_symbol) : ty :=
+    match s with
     | CONTRADICTION => \ty( o )
     | NEGATION => \ty( o -> o )
     | CONJUNCTION => \ty( o -> o -> o )
@@ -109,10 +99,42 @@ Module FirstOrderModalLogic.
     | EQUAL => \ty( i -> i -> o )
     | BOX => \ty( o -> o )
     | DIA => \ty( o -> o )
-    | FuncSym fsym_id => nat_rec (fun _ => ty) \ty( i ) (fun _ ty1 => \ty( i -> ty1 )) (arity_env.(func_arity) fsym_id)
-    | PredSym psym_id => nat_rec (fun _ => ty) \ty( o ) (fun _ ty1 => \ty( i -> ty1 )) (arity_env.(pred_arity) psym_id)
     end
   .
+
+  Definition arity : Set :=
+    nat
+  .
+
+  Record language_signature : Set :=
+    { func_arity_env : forall f_id : nat, option arity
+    ; pred_arity_env : forall p_id : nat, option arity
+    }
+  .
+
+  Inductive symbol (lsig : language_signature) : Set :=
+  | PrimSym (s : logical_symbol) : symbol lsig
+  | FuncSym (fsym_id : {f_id : nat | lsig.(func_arity_env) f_id <> None}) : symbol lsig
+  | PredSym (psym_id : {p_id : nat | lsig.(pred_arity_env) p_id <> None}) : symbol lsig
+  .
+
+  Arguments PrimSym {lsig}.
+  Arguments FuncSym {lsig}.
+  Arguments PredSym {lsig}.
+
+  Inductive tm (lsig : language_signature) : Set :=
+  | VAR (x : ivar) : tm lsig
+  | CON (c : symbol lsig) : tm lsig
+  | APP (t1 : tm lsig) (t2 : tm lsig) : tm lsig
+  | LAM (y : ivar) (t1 : tm lsig) : tm lsig
+  .
+
+  Arguments VAR {lsig}.
+  Arguments CON {lsig}.
+  Arguments APP {lsig}.
+  Arguments LAM {lsig}.
+
+  Section SEMANTICS_OF_FIRST_ORDER_MODAL_LOGIC.
 
   Variable Univ : Type.
 
@@ -142,56 +164,15 @@ Module FirstOrderModalLogic.
     end
   .
 
-  Variable arity_env : language_arity_env.
-
-  Inductive typeOf : tm -> ty -> Type :=
-  | VAR_typeOf (x : ivar) : typeOf (VAR x) \ty( i )
-  | CON_typeOf (c : symbol) : typeOf (CON c) (get_ty_of_symbol arity_env c)
-  | APP_typeOf (t1 : tm) (t2 : tm) (ty1 : ty) (ty2 : ty) (H_typeOf_t1 : typeOf t1 \ty( ty1 -> ty2 )) (H_typeOf_t2 : typeOf t2 \ty( ty1 )) : typeOf (APP t1 t2) ty2
-  | LAM_typeOf (y : ivar) (t1 : tm) (ty1 : ty) (H_typeOf_t1 : typeOf t1 \ty( ty1 )) : typeOf (LAM y t1) \ty( i -> ty1 )
-  .
-
-  Section EVALUATION_FOR_FUNC.
-
-  Variable interprete0_func : forall fsym_id : nat, Worlds -> interprete0_ty (get_ty_of_symbol arity_env (FuncSym fsym_id)).
-
-  Definition interpreteW_func (fsym_id : nat) : interpreteW_ty (get_ty_of_symbol arity_env (FuncSym fsym_id)) :=
-    nat_rect
-    (fun arity => (Worlds -> interprete0_ty (nat_rec (fun _ => ty) \ty( i ) (fun _ ty1 => \ty( i -> ty1 )) arity)) -> interpreteW_ty (nat_rec (fun _ => ty) \ty( i ) (fun _ ty1 => \ty( i -> ty1 )) arity))
-    (fun var_w => var_w)
-    (fun arity IH fun_by_w arg_by_w => IH (fun w => fun_by_w w (arg_by_w w)))
-    (func_arity arity_env fsym_id)
-    (interprete0_func fsym_id)
-  .
-
-  End EVALUATION_FOR_FUNC.
-
-  Section EVALUATION_FOR_PRED.
-
-  Variable interprete0_pred : forall psym_id : nat, Worlds -> interprete0_ty (get_ty_of_symbol arity_env (PredSym psym_id)).
-
-  Definition interpreteW_pred (psym_id : nat) : interpreteW_ty (get_ty_of_symbol arity_env (PredSym psym_id)) :=
-    nat_rect
-    (fun arity => (Worlds -> interprete0_ty (nat_rec (fun _ => ty) \ty( o ) (fun _ ty1 => \ty( i -> ty1 )) arity)) -> interpreteW_ty (nat_rec (fun _ => ty) \ty( o ) (fun _ ty1 => \ty( i -> ty1 )) arity))
-    (fun var_w => var_w)
-    (fun arity IH fun_by_w arg_by_w => IH (fun w => fun_by_w w (arg_by_w w)))
-    (pred_arity arity_env psym_id)
-    (interprete0_pred psym_id)
-  .
-
-  End EVALUATION_FOR_PRED.
+  Section SEMANTICS_OF_LOGICAL_SYMBOLS_IN_FIRST_ORDER_MODAL_LOGIC.
 
   Variable accessibility_relation : ensemble (Worlds * Worlds).
 
-  Local Notation " w1 '`is_accessible_to`' w2 " := (accessibility_relation (w1, w2)) (at level 70, no associativity) : type_scope.
+  Local Notation " w1 '`is_accessible_to`' w2 " := (member (w1, w2) accessibility_relation) (at level 70, no associativity) : type_scope.
 
-  Variable func_env : forall fsym_id : nat, Worlds -> interprete0_ty (get_ty_of_symbol arity_env (FuncSym fsym_id)).
-
-  Variable pred_env : forall psym_id : nat, Worlds -> interprete0_ty (get_ty_of_symbol arity_env (PredSym psym_id)).
-
-  Definition interpreteW_symbol (c : symbol) : interpreteW_ty (get_ty_of_symbol arity_env c) :=
-    match c with
-    | CONTRADICTION => fun w => False
+  Definition interpreteW_logical (s : logical_symbol) : interpreteW_ty (get_ty_of_logical_symbol s) :=
+    match s with
+    | CONTRADICTION => fun _ => False
     | NEGATION => fun wP1 w => ~ wP1 w
     | CONJUNCTION => fun wP1 wP2 w => wP1 w /\ wP2 w
     | DISJUNCTION => fun wP1 wP2 w => wP1 w \/ wP2 w
@@ -202,12 +183,65 @@ Module FirstOrderModalLogic.
     | EQUAL => fun x_val y_val w => x_val w = y_val w
     | BOX => fun wP1 w => forall w' : Worlds, w `is_accessible_to` w' -> wP1 w'
     | DIA => fun wP1 w => exists w' : Worlds, w `is_accessible_to` w' /\ wP1 w'
-    | FuncSym fsym_id => interpreteW_func func_env fsym_id
-    | PredSym psym_id => interpreteW_pred pred_env psym_id
     end
   .
 
-  Fixpoint interpreteW_tm (ivar_env : ivar -> wUniv) (tm_expr : tm) (ty_expr : ty) (H : typeOf tm_expr ty_expr) {struct H} : interpreteW_ty ty_expr :=
+  End SEMANTICS_OF_LOGICAL_SYMBOLS_IN_FIRST_ORDER_MODAL_LOGIC.
+
+  Variable lsig : language_signature.
+
+  Definition get_ty_of_symbol (c : symbol lsig) : ty :=
+    match c with
+    | PrimSym s => get_ty_of_logical_symbol s
+    | FuncSym fsym_id => nat_rec (fun _ => ty) \ty( o ) (fun _ ty1 => \ty( i -> ty1 )) (fromJust (lsig.(func_arity_env) (proj1_sig fsym_id)) (proj2_sig fsym_id))
+    | PredSym psym_id => nat_rec (fun _ => ty) \ty( o ) (fun _ ty1 => \ty( i -> ty1 )) (fromJust (lsig.(pred_arity_env) (proj1_sig psym_id)) (proj2_sig psym_id))
+    end
+  .
+
+  Inductive typeOf : tm lsig -> ty -> Type :=
+  | VAR_typeOf (x : ivar) : typeOf (VAR x) \ty( i )
+  | CON_typeOf (c : symbol lsig) : typeOf (CON c) (get_ty_of_symbol c)
+  | APP_typeOf (t1 : tm lsig) (t2 : tm lsig) (ty1 : ty) (ty2 : ty) (H_typeOf_t1 : typeOf t1 \ty( ty1 -> ty2 )) (H_typeOf_t2 : typeOf t2 \ty( ty1 )) : typeOf (APP t1 t2) ty2
+  | LAM_typeOf (y : ivar) (t1 : tm lsig) (ty1 : ty) (H_typeOf_t1 : typeOf t1 \ty( ty1 )) : typeOf (LAM y t1) \ty( i -> ty1 )
+  .
+
+  Definition interpreteW_func (fsym_id : {f_id : nat | lsig.(func_arity_env) f_id <> None}) :
+    (Worlds -> interprete0_ty (get_ty_of_symbol (FuncSym fsym_id))) ->
+    interpreteW_ty (get_ty_of_symbol (FuncSym fsym_id)).
+  Proof.
+    simpl.
+    generalize (fromJust (lsig.(func_arity_env) (proj1_sig fsym_id)) (proj2_sig fsym_id)).
+    induction a as [| a IH].
+    - exact (fun val_w => val_w).
+    - exact (fun fun_w arg_w => IH (fun w => fun_w w (arg_w w))).
+  Defined.
+
+  Definition interpreteW_pred (psym_id : {p_id : nat | lsig.(pred_arity_env) p_id <> None}) :
+    (Worlds -> interprete0_ty (get_ty_of_symbol (PredSym psym_id))) ->
+    interpreteW_ty (get_ty_of_symbol (PredSym psym_id)).
+  Proof.
+    simpl.
+    generalize (fromJust (lsig.(pred_arity_env) (proj1_sig psym_id)) (proj2_sig psym_id)).
+    induction a as [| a IH].
+    - exact (fun val_w => val_w).
+    - exact (fun fun_w arg_w => IH (fun w => fun_w w (arg_w w))).
+  Defined.
+
+  Variable func_env : forall fsym_id : {f_id : nat | lsig.(func_arity_env) f_id <> None}, Worlds -> interprete0_ty (get_ty_of_symbol (FuncSym fsym_id)).
+
+  Variable pred_env : forall psym_id : {p_id : nat | lsig.(pred_arity_env) p_id <> None}, Worlds -> interprete0_ty (get_ty_of_symbol (PredSym psym_id)).
+
+  Variable accessibility_relation : ensemble (Worlds * Worlds).
+
+  Definition interpreteW_symbol (c : symbol lsig) : interpreteW_ty (get_ty_of_symbol c) :=
+    match c with
+    | PrimSym s => interpreteW_logical accessibility_relation s
+    | FuncSym fsym_id => interpreteW_func fsym_id (func_env fsym_id) 
+    | PredSym psym_id => interpreteW_pred psym_id (pred_env psym_id)
+    end
+  .
+
+  Fixpoint interpreteW_tm (ivar_env : ivar -> wUniv) (tm_expr : tm lsig) (ty_expr : ty) (H : typeOf tm_expr ty_expr) {struct H} : interpreteW_ty ty_expr :=
     match H with
     | VAR_typeOf x => ivar_env x
     | CON_typeOf c => interpreteW_symbol c
@@ -216,6 +250,6 @@ Module FirstOrderModalLogic.
     end
   .
 
-  End EVALUATION.
+  End SEMANTICS_OF_FIRST_ORDER_MODAL_LOGIC.
 
 End FirstOrderModalLogic.
